\documentclass{article}
\usepackage{amsmath}

\begin{document}
	
	\begin{equation*}
		F = F_{bulk} = \int (f_{splay} + f_{twist} + f_{bend}) d^3 \vec{r}
	\end{equation*}

	\begin{equation*}
	= \int\frac{1}{2}(K_1(\nabla\cdot\vec{n})^2 + K_2(\vec{n}\cdot(\nabla\times\vec{n}))^2+K_3(\vec{n}\times(\nabla\times\vec{n}))^2))d^3\vec{r}
	\end{equation*}

	\begin{equation*}
		U_{GB} (\hat{u_i},\hat{u_j},\vec{r_{ij}})= 4\epsilon(\hat{u_i},\hat{u_j},\vec{r_{ij}})\left(\frac{1}{R^{12}(\hat{u_i},\hat{u_j},\vec{r_{ij}})}-\frac{1}{R^{6}(\hat{u_i},\hat{u_j},\vec{r_{ij}})}\right)
	\end{equation*}

	\begin{equation*}
		U_{sphere} (\hat{u}, \vec{r}) = 4\epsilon_0\left(\frac{1}{R^{18}(\hat{u}, \vec{r})}\right)-W\frac{(\hat{r}\cdot\hat{u})^6}{r^6}
	\end{equation*}
	
	\begin{equation*}
		Q =\frac{1}{N}\sum_{i}^{N}(u_{\alpha}^{(i)}u_{\beta}^{(i)}-\frac{1}{3}\delta_{\alpha\beta}) = \frac{1}{N}\sum_{i}^{N}
	\[
	\begin{bmatrix}
		u_x^{(i)}u_x^{(i)}-\frac{1}{3} & u_x^{(i)}u_y^{(i)} & u_x^{(i)}u_z^{(i)} \\
		u_y^{(i)}u_x^{(i)} & u_y^{(i)}u_y^{(i)}-\frac{1}{3} & u_y^{(i)}u_z^{(i)} \\
		u_z^{(i)}u_x^{(i)} & u_z^{(i)}u_y^{(i)} & u_z^{(i)}u_z^{(i)}-\frac{1}{3} 

	\end{bmatrix}
	\]
	\end{equation*}

	\begin{equation*}
		2\pi s = \oint d\theta
	\end{equation*}

	\begin{equation*}
		v_i(t+\frac{\Delta t}{2}) = v_i(t) + a_i(t)\frac{\Delta t}{2}
	\end{equation*}

	\begin{equation*}
		x_i(t+\Delta t) = x_i(t) + v_i(t+\frac{\Delta t}{2})\Delta t
	\end{equation*}
	
	\begin{equation*}
		v_i(t+\Delta t) = v_i(t+\frac{\Delta t}{2}) + a_i(t+\frac{\Delta t}{2})\frac{\Delta t}{2}
	\end{equation*}

	\begin{equation*}
		e_i(t+\Delta t) = e_i(t) + u_i(t + \frac{\Delta t}{2})\Delta t + \lambda e_i(t) \Delta t
	\end{equation*}

	\begin{equation*}
		u_i(t+\Delta t) = u_i(t+\frac{\Delta t}{2}) + \alpha_i(t+\Delta t)\frac{\Delta t}{2} + \tilde{\lambda} e_i(t+\Delta t)\frac{\Delta t}{2}
	\end{equation*}

\end{document}
